theories/Vector.v
@@ -14,6 +14,9 @@ Arguments vector : clear implicits.
 
 Notation bitvec := (vector bool).
 
+Declare Scope vector_scope.
+Delimit Scope vector_scope with vector.
+Bind Scope vector_scope with vector.
 Notation "[| |]" := {| vector_list := []; vector_wf := eq_refl |} (format "[| |]").
 Notation "[| x |]" := {| vector_list := [x]; vector_wf := eq_refl |}.
 Notation "[| x ; y ; .. ; z |]" := {| vector_list := cons x (cons y .. [z] ..); vector_wf := eq_refl |}.
@@ -22,6 +25,40 @@ Register vector as vcpu.vector.type.
 Register Build_vector as vcpu.vector.constructor.
 Register vector_list as vcpu.vector.list.
 Register vector_wf as vcpu.vector.wf.
+
+Definition mk_vector {A n} v_list v_wf : vector A n := {|
+  vector_list := v_list;
+  vector_wf := normalize_eq_binnat _ _ v_wf;
+|}.
+
+Lemma mk_vector_ext :
+  forall {A n} (v_list : list A) (v_wf_1 v_wf_2 : length_bin v_list = n),
+  mk_vector v_list v_wf_1 = mk_vector v_list v_wf_2.
+Proof.
+  intros A n v_list v_wf_1 v_wf_2. unfold mk_vector. f_equal. apply normalize_eq_binnat_ext.
+Qed.
+
+Lemma mk_vector_ext_all :
+  forall {A n} (v_list_1 v_list_2 : list A)
+  (v_wf_1 : length_bin v_list_1 = n) (v_wf_2 : length_bin v_list_2 = n),
+  v_list_1 = v_list_2 ->
+  mk_vector v_list_1 v_wf_1 = mk_vector v_list_2 v_wf_2.
+Proof.
+  intros A n v_list_1 v_list_2 v_wf_1 v_wf_2 H. subst v_list_2. apply mk_vector_ext.
+Qed.
+
+Lemma mk_vector_eq_refl :
+  forall {A} (l : list A),
+  mk_vector l eq_refl = {| vector_list := l; vector_wf := eq_refl |}.
+Proof.
+  intros A l. unfold mk_vector. f_equal. apply normalize_eq_binnat_eq_refl.
+Qed.
+
+Definition vector_normalize {A n} (v : vector A n) : vector A n := mk_vector (vector_list v) (vector_wf v).
+
+Definition vector_similar {A n1 n2} (v1 : vector A n1) (v2 : vector A n2) := vector_list v1 = vector_list v2.
+
+Infix "~=" := vector_similar (at level 70) : type_scope.
 
 #[program] Definition vector_head {A n} (v : vector A (N.succ n)) : A :=
   match vector_list v with
@@ -48,14 +85,34 @@ Definition vector_dest {A n} (v : vector A (N.succ n)) : A * vector A n :=
 
 Register vector_dest as vcpu.vector.dest.
 
-#[program] Definition vector_app {A n1 n2} (v1 : vector A n1) (v2 : vector A n2) : vector A (n1 + n2) := {|
-  vector_list := vector_list v1 ++ vector_list v2;
-|}.
+#[program] Definition vector_app {A n1 n2} (v1 : vector A n1) (v2 : vector A n2) : vector A (n1 + n2) :=
+  mk_vector (vector_list v1 ++ vector_list v2) _.
 Next Obligation.
   intros A n1 n2 v1 v2. rewrite length_bin_app. rewrite ? vector_wf. auto.
 Qed.
 
+Infix "++" := vector_app : vector_scope.
+
 Register vector_app as vcpu.vector.app.
+
+Lemma vector_app_mk_vector :
+  forall A n1 n2 (v_list_1 v_list_2 : list A)
+    (v_wf_1 : length_bin v_list_1 = n1) (v_wf_2 : length_bin v_list_2 = n2),
+  ((mk_vector v_list_1 v_wf_1) ++ (mk_vector v_list_2 v_wf_2))%vector =
+    mk_vector (v_list_1 ++ v_list_2)
+      (vector_app_obligation_1 _ _ _(mk_vector v_list_1 v_wf_1) (mk_vector v_list_2 v_wf_2)).
+Proof.
+  intros A n1 n2 v_list_1 v_list_2 v_wf_1 v_wf_2. unfold vector_app. apply mk_vector_ext.
+Qed.
+
+Definition vector_select_bin_vec {A n} (values : vector A n) indices default : vector A (length_bin indices) :=
+  mk_vector (list_select_bin (vector_list values) indices default) (length_bin_list_select_bin _ _ _).
+
+#[program] Definition vector_map {A B n} f (v : vector A n) : vector B n :=
+  mk_vector (List.map f (vector_list v)) _.
+Next Obligation.
+  intros A B n f v. rewrite length_bin_list_map. apply (vector_wf v).
+Qed.
 
 Unset Program Cases.
 
